failed hack at printing

Printing.dfy
@@ -213,15 +213,137 @@ method printmappingIsIsomorphic(m: vmap<Object,Object>, o : Object, os : set<Obj
 
 
 
-
 function fmtnickset(Y: set<Object>) : string
+ reads Y`nick
  {
-  //var Y := X;
-  if (Y == {}) then ("") else (
-      var y : Object :| y in Y && (forall z <- Y :: y.nick <= z.nick );
-      y.nick + " " + fmtnickset( Y - {y} ) )
-  } 
+   "FUCKOFF"
+//    fmtsetstr( set y <- Y :: y.nick )
+ } 
 
+
+lemma {:axiom} StrLEQ1(a : string,  b : string)
+  ensures (strLEQ(a, b) && strLEQ(b, a)) <==> (a == b)
+
+lemma {:axiom}  StrLEQ2(a : string,  b : string, c : string)
+  ensures (strLEQ(a, b) && strLEQ(b, c)) ==> strLEQ(a, c)
+
+lemma {:axiom} StrLEQ3(a : string,  b : string)
+  ensures  strLEQ(a, b) || strLEQ(b, a)
+
+lemma {:axiom} StrLEQ4(a : string)
+  ensures  strLEQ(a, a)
+
+
+
+
+ghost function anyOneOf(s: set<string>) : string
+  requires |s| > 0
+{
+  ExtractFromNonEmptySet(s)
+ }
+
+
+predicate IAMTheRessurection(s: set<string>, m : string) 
+{
+  m in s && forall x <- s :: strLEQ(m, x)
+}
+
+
+
+
+// ghost function IAMTheLife(s: set<string>) : (m : string) 
+//   requires |s| > 0
+//   ensures  IAMTheRessurection(s,m)
+//   {
+//    var mm :| mm in s && IAMTheRessurection(s,mm); mm
+//   }
+// 
+// 
+// lemma ThereIsOneTrueFaith(s: set<string>)
+//   requires |s| > 0
+//   ensures exists m <- s :: IAMTheRessurection(s, m)
+//   {
+//     if (|s| == 1) 
+//        {
+//         var m := theOneAndOnly(s);
+//         assert strLEQ(m,m);
+//         assert forall x <- s :: x == m && strLEQ(x,m);
+//         assert IAMTheRessurection(s, m);
+//         assert exists m <- s :: IAMTheRessurection(s, m);       
+//        }
+//     else 
+//     {
+//       assert |s| > 1;
+//       var guess :| guess in s; 
+//       var rest  := s - {guess};
+//       assert s == ({guess} + rest);
+//       ThereIsOneTrueFaith(rest);
+//       var bestOfTHeRest := IAMTheLife(rest);
+//       assert IAMTheRessurection(rest, bestOfTHeRest);
+//       if (strLEQ(guess,bestOfTHeRest))
+//          {
+//           assert s == ({guess} + rest);
+//           assert IAMTheRessurection(s, guess);
+//           assert exists m <- s :: IAMTheRessurection(s, m);
+//          } else {
+//           assert s == ({guess} + rest);
+//           assert IAMTheRessurection(s, bestOfTHeRest);
+//           assert exists m <- s :: IAMTheRessurection(s, m);          
+//          }
+//     assert exists m <- s :: IAMTheRessurection(s, m);          
+//     }
+//  assert exists m <- s :: IAMTheRessurection(s, m);          
+// }
+
+function theOneAndOnly(s: set<string>) : string
+  requires |s| == 1
+{
+  ExtractFromSingleton(s)
+}
+
+  
+
+// 
+// function fmtsetstr(Y: set<string>) : string
+//  {
+//   if (Y == {}) then ("") else (
+//       var y : string :| y in Y && (forall z <- Y :: strLEQ(y,z) );
+//       y + " " + fmtsetstr( Y - {y} ) )
+//   } 
+
+
+
+lemma TEST()
+  ensures strLEQ("","")
+  ensures strLEQ("3","3")
+  ensures strLEQ("12345","12345")  
+  ensures strLEQ("","oiwr")
+  ensures strLEQ("abc", "abcde")
+  ensures strLEQ("a", "z")
+  ensures strLEQ("ab", "z")
+  ensures not(strLEQ("abc","ab"))
+  ensures not(strLEQ("abzd", "abcd"))
+{}
+
+lemma STRLEQEQ(s : string) 
+ ensures strLEQ(s,s)
+ {
+  if (|s| == 0)  {assert strLEQ("",""); return; }
+
+  assert |s| > 0;
+  assert not (s[0] < s[0]);
+  assert (s[0] == s[0]);
+assert (strLEQ(s[1..], s[1..]));
+
+ }
+
+predicate strLEQ(l : string, r : string) 
+{
+  || (|l| == 0)
+  || (&& (|r| > 0) 
+      && (|| (l[0] < r[0]) 
+          || ((l[0] == r[0]) && (strLEQ(l[1..], r[1..])))))
+}
 
 
 function fmtseqstr(Y: seq<string>) : string  //isnt this just a flatten?
@@ -230,3 +352,184 @@ function fmtseqstr(Y: seq<string>) : string  //isnt this just a flatten?
   if (Y == []) then ("") else (
        Y[0] + " " + fmtseqstr( Y[1..] ) )
   } 
+// 
+// lemma MSSFX(s : set<string>) 
+//  requires |s| > 0
+//  ensures  exists m <- s :: forall x <- s :: strLEQ(m, x)
+//  {
+//   //  var v :| IAMTheRessurection(s, v);
+//   //  MSSFF(s, v);
+//   //  assert exists mm <- s :: ((forall x <- s :: strLEQ(mm, x)) ==> (v == mm));
+// 
+//   assert |s| > 0;
+//   assert exists m :: m in s;
+//   assert exists m <- s, x <- s :: m == x;
+// 
+//   forall m <- s, x <- s ensures ((m == x) ==> (strLEQ(m,x)))
+//     {
+//       if (m == x)
+//         {
+//           assert (strLEQ(m,x)) == (strLEQ(x,x)) == (strLEQ(m,m)) == (strLEQ(x,m)) == true 
+//             by {
+//               STRLEQEQ(m);
+//             }
+//           assert ((m == x) ==> (strLEQ(m,x)));
+//         }
+//         else 
+//         {
+//           assert m != x;
+//           assert ((m == x) ==> (strLEQ(m,x)));
+//         }
+//       assert ((m == x) ==> (strLEQ(m,x)));
+//     }
+//     
+// 
+//   assert exists m <- s :: exists x <- s ::   strLEQ(m,x);
+//   assert forall x <- s :: exists m <- s ::   strLEQ(m,x);
+// 
+// //  assert  exists m <- s :: IAMTheRessurection(s,m); //:: forall x <- s :: strLEQ(m, x);
+// 
+//  assert  exists m <- s :: forall x <- s :: strLEQ(m, x);
+//  }
+
+
+lemma MSSFF(s : set<string>, m : string) 
+ requires |s| > 0
+ requires IAMTheRessurection(s, m)
+ ensures  forall x <- s :: strLEQ(m, x)
+ ensures  exists mm <- s :: ((forall x <- s :: strLEQ(mm, x)) ==> (m == mm))
+ ensures  exists m <- s :: forall x <- s :: strLEQ(m, x)
+ {}
+
+// function mss(s : set<string>) : (m : string)
+//  requires |s| > 0
+//  ensures  IAMTheRessurection(s,m)
+// {
+//   var x :| x in s && IAMTheRessurection(s,x);
+//   x
+// }
+// by method {
+//  m := minsetstr(s);
+// }
+
+method minsetstr(s : set<string>) returns (m : string)
+  requires |s| > 0
+  ensures  IAMTheRessurection(s,m)
+{
+  var t := s;
+  m :| m in s; 
+  var z := {m};
+  assert strLEQ(m,m) by { STRLEQEQ(m); }
+  assert m in z;
+  assert forall x <- z :: strLEQ(m,x);
+  assert IAMTheRessurection(z,m);
+             
+  t := t - {m};
+
+  while t != {}
+    decreases t
+    invariant IAMTheRessurection(z,m)
+    invariant s == t + z
+  {
+    var y: string;
+    y :| y in t;
+
+assert IAMTheRessurection(z,m);
+assert (m in z && forall x | x in z && strLEQ(x, m) :: strLEQ(m, x));
+
+
+    if (strLEQ(y, m)) {
+      assert IAMTheRessurection(z,m);      
+      // assert (forall x | x in (z) :: strLEQ(m, x));  
+      forall x <- (z) ensures ( strLEQ(m, x) )   {  }
+      assert strLEQ(y, m);
+      forall x <- (z) ensures ( strLEQ(y, x) )   { StrLEQ2(y,m,x); }
+
+      // assert (forall x | x in (z) :: strLEQ(y, x));  
+      // assert (forall x | x in (z+{y}) :: strLEQ(y, x));        
+      //assert (m in (z) && forall x | x in (z+{y}) && strLEQ(x, y) ::  strLEQ(y, x));
+      assert strLEQ(y,y) by { STRLEQEQ(y); }
+      assert (y in (z+{y}) && forall x <- (z+{y}) :: strLEQ(y, x));       
+      m := y;
+      assert IAMTheRessurection(z+{y},m);
+     }
+    else 
+    {
+      assert not(strLEQ(y, m));
+      assert strLEQ(m, y) by { StrLEQ3(y,m); }
+      assert IAMTheRessurection(z,m);
+      assert (m in (z+{y})  && forall x <- (z+{y}) :: strLEQ(m, x));
+      assert IAMTheRessurection((z+{y}),m);
+    }
+
+
+    t := t - {y};
+    z := z + {y};
+
+    assert IAMTheRessurection(z,m);
+  }
+
+  assert IAMTheRessurection(t + z, m);
+  assert IAMTheRessurection(s, m);
+}
+
+
+
+
+
+  /** Any totally-ordered set contains a unique minimal (equivalently, least) element. */
+  lemma LemmaFindUniqueMinimal(s: set<string>) returns (min: string)
+    requires |s| > 0 // TotalOrdering(R)
+    ensures IAMTheRessurection(s, min) // && (forall min' <- s | IAMTheRessurection(s, min') :: min == min')
+  {
+    var x :| x in s;
+    if s == {x} {
+      min := x;
+      StrLEQ4(x); 
+      StrLEQ4(min); 
+    assert IAMTheRessurection({x}, min);
+    assert IAMTheRessurection(s, min);
+    // StrLEQ1(min, x);
+    // StrLEQ3(min, x);
+    // StrLEQ4(min);
+    // StrLEQ4(x);
+    } else {
+      var min' := LemmaFindUniqueMinimal(s - {x});
+      assert IAMTheRessurection(s - {x}, min');
+      assert forall q <- (s - {x}) :: strLEQ(min', q);
+      assert min' in (s - {x});
+      StrLEQ3(min', x);
+      if
+      case strLEQ(min', x) => 
+          assert forall q <- (s - {x}) :: strLEQ(min', q);
+          assert strLEQ(min', x);
+          assert forall q <- (s - {x} + {x}) :: strLEQ(min', q);
+          assert (s - {x}) + {x} == s;
+          assert forall q <- (s) :: strLEQ(min', q);
+          min := min'; 
+          assert forall q <- (s) :: strLEQ(min', q);
+          assert min in s;
+          assert forall q <- s :: strLEQ(min, q);
+          assert IAMTheRessurection(s, min);  
+
+      case strLEQ(x, min') => min := x;
+          assert forall q <- (s - {x}) :: strLEQ(min', q);
+          forall q <- (s - {x}) ensures strLEQ(min, q)  
+            {  
+              assert strLEQ(min', q);
+              assert strLEQ(min, min');
+              StrLEQ2(min, min',q);
+            }
+          StrLEQ4(x); 
+          assert min == x;
+          assert strLEQ(min, x);
+          StrLEQ4(min);  
+          assert (s - {x}) + {x} == s;
+          assert IAMTheRessurection(s, min);  
+    }
+    assert IAMTheRessurection(s, min); 
+  }
+
+
+
+
